ok
git-svn-id: svn://scm.gforge.inria.fr/svn/cfml@31 ba02c806-7d2b-4818-9a48-35b22e6bdc79

okasaki/CatenableListImpl.ml
@@ -1,10 +1,63 @@
 open Okasaki
 open CatenableListSig
+open QueueSig
+open BankersQueue
 
+(*module Q = BatchedQueue*)
+
+module CatenableListImpl : CatenableList =
+struct
+
+   type 'a cats = Empty | Struct of 'a * 'a cats Lazy.t BankersQueue.queue
+   type 'a cat = 'a cats
+
+   let empty = Empty
+
+   let is_empty = function 
+      | Empty -> true
+      | _ -> false
+
+   let link xs s =
+      match xs with
+      | Empty -> raise BrokenInvariant
+      | Struct (x, q) -> Struct (x, BankersQueue.snoc q s)
+   
+   let rec link_all q =
+      let t = !$ (BankersQueue.head q) in
+      let q' = BankersQueue.tail q in
+      if BankersQueue.is_empty q' 
+         then t 
+         else link t (lazy (link_all q'))
+
+   let append xs1 xs2 =
+      match xs1, xs2 with
+      | Empty, _ -> xs2
+      | _, Empty -> xs1
+      | _ -> link xs1 (lazy xs2)
+
+   let cons x xs = 
+      append (Struct (x, BankersQueue.empty)) xs
+   
+   let snoc xs x =
+      append xs (Struct (x, BankersQueue.empty))
+
+   let head = function
+      | Empty -> raise EmptyStructure
+      | Struct (x, _) -> x
+
+   let tail = function
+      | Empty -> raise EmptyStructure
+      | Struct (x, q) -> 
+         if BankersQueue.is_empty q then Empty else link_all q
+   
+end
+
+
+(*
 module CatenableListImpl (Q : Queue) : CatenableList =
 struct
 
-   type 'a cats = Empty | Struct of 'a * 'a cats Lazy.t Queue.q
+   type 'a cats = Empty | Struct of 'a * 'a cats Lazy.t Q.queue
    type 'a cat = 'a cats
 
    let empty = Empty
@@ -29,7 +82,7 @@ struct
       match xs1, xs2 with
       | Empty, _ -> xs2
       | _, Empty -> xs1
-      | _ -> link xs1 (lazy s2)
+      | _ -> link xs1 (lazy xs2)
 
    let cons x xs = 
       append (Struct (x, Q.empty)) xs
@@ -44,6 +97,7 @@ struct
    let tail = function
       | Empty -> raise EmptyStructure
       | Struct (x, q) -> 
-         if Q.empty q then Empty else link_all q
+         if Q.is_empty q then Empty else link_all q
    
 end
+*)
